going into beta-value path

sf/StlcProp.v
@@ -6,6 +6,7 @@ Require Import Stlc.
 Require Import Smallstep.
 Module STLCProp.
 Import STLC.
+Require Import Omega.
 
 (** In this chapter, we develop the fundamental theory of the Simply
     Typed Lambda Calculus -- in particular, the type safety
@@ -1439,6 +1440,31 @@ assert (tapp x0 t2 ==> tapp y0 t2).
 eapply multi_step; eauto.
 Qed.
 
+Lemma succ_multi_step : forall t t',
+  t ==>* t' -> tsucc t ==>* tsucc t'.
+Proof.
+intros. induction H.
+- auto.
+- eapply multi_step. eauto. eauto.
+Qed.
+
+Lemma pred_multi_step : forall t t',
+  t ==>* t' -> tpred t ==>* tpred t'.
+Proof.
+intros. induction H.
+- auto.
+- eapply multi_step. eauto. eauto.
+Qed.
+
+
+(*Marked! We're working here!*)
+Lemma mult_multi_step : forall t1 t1' t2 t2',
+  t ==>* t' -> tsucc t ==>* tsucc t'.
+Proof.
+intros. induction H.
+- auto.
+- eapply multi_step. eauto. eauto.
+Qed.
 Lemma canonical_forms_serious : forall t T1 T2,
   empty |- t \in (TArrow T1 T2) ->
   exists t' x u, t' = tabs x T1 u /\ t ==>* t'.
@@ -1547,216 +1573,68 @@ Proof. induction t; intros.
   reflexivity.
 Qed.
 
-(*if we can prove that the complexity of a term always decrease
-by one after every reduction step, we win!*)
 
-(*Inductive complex: tm -> nat -> Prop :=
-  | C_Var : forall i,
-    complex (tvar i) 0
-  | C_App: forall t1 t2 n1 n2 x T u,
-    complex t2 n2 -> complex t1 n1 ->
-    t1 ==>* (tabs x T u) ->
-    complex (tapp t1 t2) (n1 + (afi_count x u)*n2 + 1)
 
-  | C_Abs: forall i T t,
-    complex (tabs i T t) 0
-    (*I think this makes the most sense*)
+(*beta value: determine how many beta-reduction must
+be done in order for the term to reach a value*)
+Inductive bval : tm -> nat -> Prop :=
+  | B_Var: forall i,
+    bval (tvar i) 0
+  | B_App: forall t1 t2 n1 n2,
+    bval t1 n1 -> bval t2 n2 ->
+    bval (tapp t1 t2) (1 + n1 + n2)
+  | B_Abs: forall i T t n,
+    bval t n ->
+    bval (tabs i T t) n
 
-  | C_Nat: forall n, complex (tnat n) 0
-  | C_Succ: forall t n,
-    complex t n ->
-    complex (tsucc t) (n + 1)
-  | C_Pred: forall t n,
-    complex t n ->
-    complex (tsucc t) (n + 1)
-  | C_Mult: forall t1 t2 n1 n2,
-    complex t1 n1 -> complex t2 n2 ->
-    complex (tmult t1 t2) (n1 + n2 + 1)
-  | C_If0_True: forall t1 t2 t3 n1 n2,
-    complex t1 n1 -> complex t2 n2 ->
+  | B_Nat: forall m,
+    bval (tvar m) 0
+  | B_Succ: forall t n,
+    bval t n ->
+    bval (tsucc t) n
+  | B_Pred: forall t n,
+    bval t n ->
+    bval (tpred t) n
+  | B_Mult: forall t1 t2 n1 n2,
+    bval t1 n1 -> bval t2 n2 ->
+    bval (tmult t1 t2) (n1 + n2)
+  | B_If0_True: forall t1 t2 t3 n1 n2,
     tif0 t1 t2 t3 ==>* t2 ->
-    complex (tif0 t1 t2 t3) (n1 + n2 + 1)
-  | C_If0_False: forall t1 t2 t3 n1 n3,
-    complex t1 n1 -> complex t3 n3 ->
+    bval t1 n1 -> bval t2 n2 ->
+    bval (tif0 t1 t2 t3) (n1 + n2)
+  | B_If0_False: forall t1 t2 t3 n1 n3,
     tif0 t1 t2 t3 ==>* t3 ->
-    complex (tif0 t1 t2 t3) (n1 + n3 + 1).
-*)
-(*This is the NEW HOPE: complexity theory*)
+    bval t1 n1 -> bval t3 n3 ->
+    bval (tif0 t1 t2 t3) (n1 + n3).
 
-(*I initially used Fixpoint computation but 
-it was just so inflexible for the tif0 case (guess what?
-now I know what they were talking about when comparing
-Fixpoint and Inductive properties, it takes a long time,
-but it was worth it!*)
+Theorem bval_0: forall t T,
+  bval t 0 -> empty |- t \in T ->
+  exists t', t ==>* t' /\ value t'.
+Proof. intros t. induction t; intros.
+- inversion H0. inversion H3.
+- inversion H.
+- exists (tabs i t t0). split; auto.
+- exists (tnat n); auto.
+- inversion H; subst. eapply IHt in H2.
 
+Focus 2. inversion H0. eauto.
 
+destruct H2. destruct H1. rename x0 into t'.
+inversion H0; subst. assert (exists n, t' = tnat n).
+{ assert (empty |- t' \in TNat).
+{ eapply preservation_multi; eauto. }
+apply canonical_forms_nat; assumption. }
 
-(*Lemma subst_order2: forall u x1 x0 s t,
-  x0 <> x1 -> value t ->
-  [x1 := [x0 := s] t] ([x0 := s] u) =
-  [x0 := s] ([x1 := t] u).
-Proof.
-intro u; induction u; intros; simpl.
-- remember (beq_id x0 i) as b0.
-remember (beq_id x1 i) as b1.
-destruct b0; destruct b1.
-  + symmetry in Heqb0. apply beq_id_true_iff in Heqb0.
-  symmetry in Heqb1. apply beq_id_true_iff in Heqb1.
-  subst. destruct H. reflexivity.
-  + simpl. rewrite <- Heqb0.
-*)
-
-
-
-(*Theorem subst_step : forall t t' x s,
-  t ==> t' -> [x := s] t ==> [x := s] t'.
-Proof.
-intros. generalize dependent x0.
-generalize dependent s.
-induction H; intros; simpl.
-- remember (beq_id x1 x0) as b10; destruct b10.
-  + symmetry in Heqb10. apply beq_id_true_iff in Heqb10.
-  subst.
-   assert (tapp (tabs x0 T t12) ([x0 := s] v2) ==>
-  [x0 := [x0 := s] v2] ( t12)).
-  { apply ST_AppAbs. apply value_subst; auto. }
-  assert ([x0 := [x0 := s] v2] t12 =
-    [x0 := s] ([x0 := v2] t12)) by (apply subst_order).
-  rewrite <- H1. auto.
+destruct H3. rename x0 into m.
+exists (tsucc (tnat m)). split.
+  + induction H1. subst. apply multi_refl.
+  assert (tsucc y0 ==>* tsucc (tnat m)).
+  { eapply IHmulti; eauto.
   
-  + assert (tapp (tabs x0 T ([x1 := s] t12)) ([x1 := s] v2) ==>
-      [x0 := [x1 := s] v2] ([x1 := s] t12)).
-    { apply ST_AppAbs. apply value_subst. assumption. }
-*)
-
-(* induction on term: stand still
-intro t; induction t; intros; subst.
-- inversion H.
-- inversion H; subst.
-  + simpl. destruct (beq_idP x0 x1).
-    * subst.
-    assert ((tapp (tabs x1 T t12) ([x1 := s] t2)) ==>
-      [x1 := ([x1 := s] t2)] t12).
-    { apply ST_AppAbs. inversion H3; subst.
-      - simpl. destruct (beq_idP x1 x0); apply v_abs.
-      - simpl. apply v_nat. }
-      
-    simpl. assert ([x1 := [x1 := s] t2] t12 =
-      [x1 := s] ([x1 := t2] t12)) by (apply subst_order).
-    rewrite <- H1. assumption.
-    
-    * assert (tapp (tabs x1 T ([x0 := s] t12)) ([x0 := s] t2) ==>
-      [x1 := [x0 := s] t2] ([x0 := s] t12)).
-    { apply ST_AppAbs. apply value_subst. assumption. }
-    
-    simpl.
-*)
-
-Require Import Omega.
-
-(*YES, I THINK THIS IS CORRECT, FIGHT ME!*)
-(*Theorem subst_complex : forall (x : id) s t nt ns,
-  complex t nt -> complex s ns ->
-  complex ([x := s] t)
-    (nt + (appears_count x t)*ns).
-Proof.
-intros x0 s t. generalize dependent x0;
-generalize dependent s; induction t; intros;
-rename x0 into x.
-- inversion H.
-- (*tapp*) simpl. inversion H; subst.
-
-assert (complex ([x := s] t1) (n1 + appears_count x
-  t1 * ns)).
-{ apply IHt1; auto. }
-clear IHt1.
-
-assert (complex ([x := s] t2) (n2 + appears_count x
-  t2 * ns)).
-{ apply IHt2; auto. }
-clear IHt2.
-
-remember (n1 + appears_count x t1 * ns) as n1'.
-remember (n2 + appears_count x t2 * ns) as n2'.
-
-assert (complex (tapp ([x := s] t1) ([x := s] t2))
-  (n1' + (appears_count x ([x := s] t1)) * n2' + 1)).
-{ eapply C_App; try assumption. }
-*)
-
-(*
-Theorem complex_value : forall v,
-  value v -> complex v 0.
-Proof.
-intros. destruct H.
-- apply C_Abs. - apply C_Nat.
-Qed.
-*)
-(*
-Theorem subst_value : forall v t x n,
-  value v -> complex t n ->
-  complex ([x := v] t) n.
-Proof.
-intros. generalize dependent n.
-assert (complex v 0) by (apply complex_value; assumption).
-induction t; intros; simpl.
-- intros. inversion H1; subst.
-simpl. destruct (beq_id x0 i).
-apply complex_value. assumption. assumption.
-- inversion H1; subst. 
-assert (complex (tapp ([x0 := v] t1) ([x0 := v] t2))
-  (n1 + afi_count x1 ([x0 := v] t1) * n2 + 1)).
-{ eapply C_App. }
-*)
 
 
 
-(*This is what I want to prove the most*)
-(*Theorem step_reduce_complex :
-  forall t t' n, t ==> t' ->
-  complex t n -> complex t' (n - 1).
-Proof. intros t; induction t; subst; intros.
-- inversion H.
-- inversion H0; subst. inversion H; subst.
-  + clear IHt1. inversion H3; subst.
-  simpl. assert (true = beq_id x0 x0)
-    by (apply beq_id_refl).
-  rewrite <- H1. simpl. assert (n1 + 0 + 1 - 1 = n1) by omega.
-  rewrite H2. simpl.
-*)
-
-
-
-
-
-
-
-Inductive complex : tm -> nat -> Prop :=
-  | Comp_ST: forall t t' n,
-    t ==> t' -> complex t' n -> complex t (n + 1)
-  | Comp_Val : forall t,
-    value t -> complex t 0.
-
-Theorem complex_0 : forall t,
-  complex t 0 -> value t.
-Proof.
-intros. inversion H. assert (forall n, n + 1 <> 0).
-{ intros; omega. }
-apply H4 in H0. inversion H0. assumption. Qed.
-
-(*
-Theorem complex_decidable : forall t T,
-  empty |- t \in T ->
-  exists n, complex t n.
-Proof.
-intros t. induction t; intros.
-- inversion H. inversion H2.
-- inversion H; subst.
-*)
-
-
-
-Theorem hatl : forall t T,
+Theorem halt : forall t T,
   empty |- t \in T ->
   exists t', value t' /\ t ==>* t'.
 Proof.
